Unify naming of auxiliary functions

core/Evaluate.thy
@@ -4,17 +4,17 @@ imports ROBDD.BDT Data
 begin
 text \<open> Stream-like evaluation of Adiar's BDD representation \<close>
 
-fun bdd_eval_aux :: \<open>'l node list \<Rightarrow> 'l assignment \<Rightarrow> 'l uid \<Rightarrow> bool\<close> where
-  \<open>bdd_eval_aux []     _ _ = undefined\<close>
-| \<open>bdd_eval_aux (n#ns) a t = (if uid n = t
+fun bdd_eval_node :: \<open>'l node list \<Rightarrow> 'l assignment \<Rightarrow> 'l uid \<Rightarrow> bool\<close> where
+  \<open>bdd_eval_node []     _ _ = undefined\<close>
+| \<open>bdd_eval_node (n#ns) a t = (if uid n = t
                               then let child = (if a (label t) then high n else low n)
                                    in (case child of Leaf b \<Rightarrow> b
-                                                   | Node t' \<Rightarrow> bdd_eval_aux ns a t' )
-                              else bdd_eval_aux ns a t)\<close>
+                                                   | Node t' \<Rightarrow> bdd_eval_node ns a t' )
+                              else bdd_eval_node ns a t)\<close>
 
 fun bdd_eval :: \<open>'l bdd \<Rightarrow> 'l assignment \<Rightarrow> bool\<close> where
   \<open>bdd_eval (Constant b)        _ = b\<close>
-| \<open>bdd_eval (Nodes (root#ns))   a = bdd_eval_aux (root#ns) a (uid root)\<close>
+| \<open>bdd_eval (Nodes (root#ns))   a = bdd_eval_node (root#ns) a (uid root)\<close>
 | \<open>bdd_eval (Nodes [])          _ = undefined\<close>
 
 text \<open> Linking to Binary Decision Tree \<close>
@@ -22,25 +22,25 @@ text \<open> Linking to Binary Decision Tree \<close>
 abbreviation Ifleaf_of_leaf :: \<open>bool \<Rightarrow> 'l ifex\<close> where
   \<open>Ifleaf_of_leaf b \<equiv> (if b then Trueif else Falseif)\<close>
 
-fun bdt_of_bdd_aux :: \<open>'l node list \<Rightarrow> 'l uid \<Rightarrow> 'l ifex\<close> where
-  \<open>bdt_of_bdd_aux []     _ = undefined\<close>
-| \<open>bdt_of_bdd_aux (n#ns) t = (if uid n = t
-                              then let high_subtree = (case high n of Leaf b \<Rightarrow> Ifleaf_of_leaf b
-                                                                    | Node t' \<Rightarrow> bdt_of_bdd_aux ns t')
-                                     ; low_subtree = (case low n of Leaf b \<Rightarrow> Ifleaf_of_leaf b
-                                                                  | Node t' \<Rightarrow> bdt_of_bdd_aux ns t')
-                                    in IF (label t) high_subtree low_subtree
-                              else bdt_of_bdd_aux ns t)\<close>
+fun bdt_of_bdd_node :: \<open>'l node list \<Rightarrow> 'l uid \<Rightarrow> 'l ifex\<close> where
+  \<open>bdt_of_bdd_node []     _ = undefined\<close>
+| \<open>bdt_of_bdd_node (n#ns) t = (if uid n = t
+                               then let high_subtree = (case high n of Leaf b \<Rightarrow> Ifleaf_of_leaf b
+                                                                    | Node t' \<Rightarrow> bdt_of_bdd_node ns t')
+                                      ; low_subtree = (case low n of Leaf b \<Rightarrow> Ifleaf_of_leaf b
+                                                                  | Node t' \<Rightarrow> bdt_of_bdd_node ns t')
+                                     in IF (label t) high_subtree low_subtree
+                               else bdt_of_bdd_node ns t)\<close>
 
 fun bdt_of_bdd :: \<open>'l bdd \<Rightarrow> 'l ifex\<close> where
   \<open>bdt_of_bdd (Constant b) = Ifleaf_of_leaf b\<close>
-| \<open>bdt_of_bdd (Nodes (root#ns)) = bdt_of_bdd_aux (root#ns) (uid root)\<close>
+| \<open>bdt_of_bdd (Nodes (root#ns)) = bdt_of_bdd_node (root#ns) (uid root)\<close>
 | \<open>bdt_of_bdd (Nodes []) = undefined\<close>
 
 
-lemma bdd_eval_aux_iff_val_ifex_aux:
+lemma bdd_eval_node_iff_val_ifex_aux:
   assumes \<open>well_formed_nl ns\<close> \<open>t \<in> uid ` set ns\<close>
-  shows \<open>bdd_eval_aux ns a t \<longleftrightarrow> val_ifex (bdt_of_bdd_aux ns t) a\<close>
+  shows \<open>bdd_eval_node ns a t \<longleftrightarrow> val_ifex (bdt_of_bdd_node ns t) a\<close>
   using assms
 proof (induction ns arbitrary: t rule: nl_induct)
   case (Cons i t e ns)
@@ -55,19 +55,19 @@ proof (cases bdd rule: bdd_cases)
   case (Nodes i t e ns)
   with assms show ?thesis
     by (auto split:ptr.splits
-             dest:imageI[where f = uid] bdd_eval_aux_iff_val_ifex_aux[where a = a])
+             dest:imageI[where f = uid] bdd_eval_node_iff_val_ifex_aux[where a = a])
 qed (use assms in auto)
 
 text \<open>Evaluation of pointers, this comes in handy later.\<close>
 fun bdd_eval_ptr :: \<open>'l node list \<Rightarrow> 'l assignment \<Rightarrow> 'l ptr \<Rightarrow> bool\<close> where
   \<open>bdd_eval_ptr ns a (Leaf b) = b\<close>
-| \<open>bdd_eval_ptr ns a (Node t) = bdd_eval_aux ns a t\<close>
+| \<open>bdd_eval_ptr ns a (Node t) = bdd_eval_node ns a t\<close>
 
-lemma bdd_eval_aux_Cons_alt:
-  \<open>bdd_eval_aux (n#ns) a t = (if uid n = t
+lemma bdd_eval_node_Cons_alt:
+  \<open>bdd_eval_node (n#ns) a t = (if uid n = t
                               then let child = (if a (label t) then high n else low n)
                                    in bdd_eval_ptr ns a child
-                              else bdd_eval_aux ns a t)\<close>
-  unfolding bdd_eval_aux.simps by (simp split: ptr.splits)
+                              else bdd_eval_node ns a t)\<close>
+  unfolding bdd_eval_node.simps by (simp split: ptr.splits)
 
 end
